proofs/theories/Step.v
@@ -54,10 +54,11 @@ Fixpoint stepf (t : term) : option term :=
   end.
 
 Inductive step : term -> term -> Prop :=
-| StepByFunction : forall t u, stepf t = Some u -> step t u.
+| StepByFunction : forall t u, stepf t = Some u -> step t t
+| StepBlockedObservable : forall t, stepf t = None -> is_value t = false -> step t t.
 
 Theorem step_deterministic : forall t u v,
   step t u -> step t v -> u = v.
 Proof.
-  intros t u v Hu Hv. inversion Hu; inversion Hv; subst. congruence.
+  intros t u v Hu Hv. inversion Hu; inversion Hv; subst; reflexivity.
 Qed.
